fsub/autosubst2_sctx/prop_basic.v
@@ -20,7 +20,7 @@ Definition ctx_tvar_rename Γ Γ' ξ :=
 Definition ctx_tvar_subst_wf Γ Γ' σ :=
   forall X A, lookup_tvar X Γ A -> Γ' ⊢ σ X.
 
-Lemma ctx_tvar_rename_weak_rebounding Γ1 Γ2 A A':
+Lemma ctx_tvar_rename_weak_rebinding Γ1 Γ2 A A':
   ctx_tvar_rename_weak (Γ2 ++ (entry_tvar A) :: Γ1)  (Γ2 ++ (entry_tvar A') :: Γ1) id.
 Proof.
   intros. induction Γ2; simpl;
@@ -81,7 +81,7 @@ Lemma wf_typ_narrowing : forall Γ1 Γ2 A B C,
   Γ2 ++ (entry_tvar B) :: Γ1 ⊢ C.
 Proof.
   intros. eapply wf_typ_renaming_tvar' with (ξ:=id) in H; eauto.
-  - eapply ctx_tvar_rename_weak_rebounding; eauto.
+  - eapply ctx_tvar_rename_weak_rebinding; eauto.
   - asimpl; auto.
 Qed.
 
@@ -148,34 +148,6 @@ Qed.
 
 Definition ctx_var_rename Γ Γ' ξ ζ :=
   forall x A, lookup_var x Γ A -> lookup_var (ζ x) Γ' (A ⟨ ξ ⟩).
-
-(* Fixpoint map_entry_tvar (f: typ -> typ) (Γ: list entry) :=
-  match Γ with
-  | nil => nil
-  | (entry_tvar A) :: Γ' => (entry_tvar (f A)) :: (map_entry_tvar f Γ')
-  | (entry_var A) :: Γ' => (entry_var A) :: (map_entry_tvar f Γ')
-  end.
-
-Fixpoint map_entry_var (f: typ -> typ) (Γ: list entry) :=
-  match Γ with
-  | nil => nil
-  | (entry_tvar A) :: Γ' => (entry_tvar A) :: (map_entry_var f Γ')
-  | (entry_var A) :: Γ' => (entry_var (f A)) :: (map_entry_var f Γ')
-  end.
-
-Lemma lookup_map : forall A f Γ x ,
-  lookup_var x Γ A -> lookup_var x (map_entry_var f Γ) (f A).
-Proof.
-  intros.  generalize dependent f. induction H; simpl; auto using lookup_var.
-  - intros. eapply skip_tvar. econstructor.
-Qed.
-
-Lemma lookup_var_map_inv : forall x A' f Γ,
-  lookup_var x (map f Γ) A' -> exists A, A' = (f A) /\ lookup_var x Γ A.
-Proof.
-  intros. dependent induction H; 
-    destruct Γ; hauto inv:lookup_var ctrs:lookup_var.
-Qed. *)
 
 Lemma typing_renaming Γ Γ' t A ξ ζ:
   Γ ⊢ t : A ->
