fsub/lngen/prop_basic.v
@@ -25,3 +25,74 @@ Proof.
   - split; pick fresh X; inst_cofinites_with X; 
     eapply lc_typ_all_exists with X; hauto.
 Qed.
+
+Lemma wf_typ_weakening Γ1 Γ2 Γ3 A :
+  (Γ3 ++ Γ1) ⊢ A ->
+  (Γ3 ++ Γ2 ++ Γ1) ⊢ A.
+Proof.
+  intros. dependent induction H; try hauto ctrs:wf_typ.
+  - eapply wf_typ_tvar; eauto. 
+  - inst_cofinites_for wf_typ_all; eauto.
+    intros.   
+    intros. inst_cofinites_with X.
+    rewrite_env (((X, entry_tvar A) :: Γ3) ++ Γ2 ++ Γ1); eauto.
+Qed.
+
+Lemma wf_typ_rebinding Γ1 Γ2 X A B B' :
+  (Γ2 ++ ((X, entry_tvar B) :: Γ1)) ⊢ A ->
+  (Γ2 ++ ((X, entry_tvar B') :: Γ1)) ⊢ A.
+Proof.
+  intros. dependent induction H; try hauto ctrs:wf_typ use:wf_typ_weakening.
+  - destruct (X == X0); subst; eauto.
+    + eapply wf_typ_tvar; eauto.
+    + eapply wf_typ_tvar with (A:=A); eauto.
+      eapply binds_remove_mid in H; eauto.
+      rewrite_env (Γ2 ++ (X ~ entry_tvar B') ++ Γ1).
+      eapply binds_weaken; eauto.
+  - inst_cofinites_for wf_typ_all; eauto.
+    intros.   
+    intros. inst_cofinites_with X.
+    rewrite_env (((X0, entry_tvar A) :: Γ2) ++ (X, entry_tvar B') :: Γ1).
+    eapply H1; eauto. simpl; eauto.
+Qed.
+
+Lemma subtyping_weakening Γ1 Γ2 Γ3 A B :
+  (Γ3 ++ Γ1) ⊢ A <: B ->
+  (Γ3 ++ Γ2 ++ Γ1) ⊢ A <: B.
+Proof.
+  intros. dependent induction H; try hauto ctrs:subtyping use:wf_typ_weakening.
+  - eapply sub_tvar_bound with (A:=A).
+    + apply binds_weaken; eauto.
+    + eauto.
+  - inst_cofinites_for sub_all.
+    + hauto use:wf_typ_weakening.
+    + eauto.
+    + intros. inst_cofinites_with X.
+      rewrite_env (((X, entry_tvar B1) :: Γ3) ++ Γ2 ++ Γ1). 
+      eapply H2; eauto. 
+Qed.
+
+Lemma subtyping_wf_typ Γ A B :
+  Γ ⊢ A <: B -> 
+  Γ ⊢ A /\ Γ ⊢ B.
+Proof.
+  intros. induction H; try hauto ctrs:wf_typ.
+  - split; inst_cofinites_for wf_typ_all; 
+    intros; inst_cofinites_with X; try hauto.
+    rewrite_env (nil ++ (X, entry_tvar A1) :: Γ). 
+    eapply wf_typ_rebinding; simpl; hauto.
+Qed.
+
+Corollary subtyping_wf_typ1 Γ A B :
+  Γ ⊢ A <: B -> 
+  Γ ⊢ A.
+Proof.
+  hauto use:subtyping_wf_typ.
+Qed.
+
+Corollary subtyping_wf_typ2 Γ A B :
+  Γ ⊢ A <: B -> 
+  Γ ⊢ B.
+Proof.
+  hauto use:subtyping_wf_typ.
+Qed.
