fsub/lngen/prop_subtyping.v
@@ -1,0 +1,87 @@
+Require Import Coq.Program.Equality.
+Require Import Lia.
+Require Import Metalib.Metatheory.
+From Hammer Require Import Tactics.
+
+From Coq Require Import ssreflect ssrfun ssrbool.
+
+Require Import fsub.lngen.def_ott.
+Require Import fsub.lngen.prop_ln.
+Require Import common.ltac_ln.
+Require Import common.prop_ln.
+Require Import fsub.lngen.def_extra.
+Require Import fsub.lngen.prop_basic.
+
+Lemma conj' (A B : Prop) : A -> (A -> B) -> A /\ B.
+Proof. tauto. Qed.
+
+Lemma subtyping_narrowing' B:
+  (forall Γ A C,  
+    uniq Γ ->
+    Γ ⊢ A <: B ->
+    Γ ⊢ B <: C ->
+    Γ ⊢ A <: C) ->
+  (forall Γ1 Γ2 X A B' C,
+    uniq (Γ2 ++ (X , entry_tvar B) :: Γ1) ->
+    (Γ2 ++ (X , entry_tvar B) :: Γ1) ⊢ A <: C ->
+    Γ1 ⊢ B' <: B ->
+    (Γ2 ++ (X , entry_tvar B') :: Γ1) ⊢ A <: C). 
+Proof. 
+  intros. dependent induction H1; try hauto ctrs:subtyping use:wf_typ_rebinding.
+  - destruct (X0 == X).
+    + subst. assert (A = B) by (hauto use:binds_exact). subst.
+      eapply sub_tvar_bound; eauto.
+      eapply H; eauto. hauto use:uniq_rebind. 
+      rewrite_env (nil ++ (Γ2 ++ (X ~ entry_tvar B')) ++ Γ1). 
+      apply subtyping_weakening; eauto.
+    + eapply sub_tvar_bound; eauto.
+      eapply binds_rebind_mid; eauto.
+  - inst_cofinites_for sub_all; eauto. 
+    + hauto ctrs:subtyping use:wf_typ_rebinding.
+    + intros. inst_cofinites_with X0.
+      rewrite_env (((X0, entry_tvar B1) :: Γ2) ++ (X, entry_tvar B') :: Γ1).
+      eapply H2; eauto. simpl; auto.
+Qed.
+
+Theorem subtyping_transitivity n:
+  forall Γ A B C,
+  size_typ B < n -> 
+  uniq Γ ->
+  Γ ⊢ A <: B ->
+  Γ ⊢ B <: C ->
+  Γ ⊢ A <: C.
+Proof.
+  induction n; intros; auto. inversion H.
+  induction H1; subst; intros; try hauto ctrs:subtyping use:subtyping_wf_typ1, subtyping_wf_typ2.
+  - inversion H2; eauto using subtyping.
+  - simpl in *. inversion H2; subst.
+    * hauto ctrs:subtyping use:subtyping_wf_typ1, subtyping_wf_typ2. 
+    * econstructor. eapply IHn; eauto. lia.
+      eapply IHn; eauto. lia.
+  - simpl in *. inversion H2; subst; eauto.
+    + eapply sub_top. inst_cofinites_for wf_typ_all.
+      * hauto ctrs:subtyping use:subtyping_wf_typ1, subtyping_wf_typ2. 
+      * intros. inst_cofinites_with X.
+        rewrite_env (nil ++ ((X, entry_tvar A1) :: Γ)).
+        eapply wf_typ_rebinding.
+        hauto ctrs:subtyping use:subtyping_wf_typ1, subtyping_wf_typ2.
+    + inst_cofinites_for sub_all. 
+      * hauto ctrs:subtyping use:subtyping_wf_typ1, subtyping_wf_typ2.
+      * eapply IHn; eauto. lia.
+      * intros. inst_cofinites_with X.
+        eapply IHn; eauto.
+        rewrite size_typ_open_typ_wrt_typ_rec_var; lia.
+        rewrite_env (nil ++ ((X, entry_tvar B0) :: Γ)).
+        eapply subtyping_narrowing'; eauto. intros.
+        eapply IHn; eauto. lia.
+Qed.
+
+Lemma subtyping_narrowing Γ1 Γ2 X A B B' C :
+  uniq (Γ2 ++ (X , entry_tvar B) :: Γ1) ->
+  (Γ2 ++ (X , entry_tvar B) :: Γ1) ⊢ A <: C ->
+  Γ1 ⊢ B' <: B ->
+  (Γ2 ++ (X , entry_tvar B') :: Γ1) ⊢ A <: C.
+Proof.
+  intros. eapply subtyping_narrowing'; eauto.
+  intros. eapply subtyping_transitivity; eauto.
+Qed.
